src/NFA.lean
@@ -2,21 +2,21 @@ import data.fintype.basic
 import data.set.lattice
 import DFA
 
+universes u v
+
 structure NFA := 
-(alphabet : Type) 
+(alphabet : Type u) 
 [alphabet_fintype : fintype alphabet]
-(state : Type)
+(state : Type v)
 [state_fintype : fintype state]
 (step : state → alphabet → set state)
-[step_dec : Π (S : state) (a : alphabet), decidable_pred (step S a)]
 (start : set state)
-[start_dec : decidable_pred start]
 (accept_states : set state)
 
 namespace NFA
 
-instance dec₁ (M : NFA) : decidable_pred M.start := M.start_dec
-instance dec₂ (M : NFA) : Π (S : M.state) (a : M.alphabet), decidable_pred (M.step S a) := M.step_dec
+@[reducible] def start_dec (M : NFA) := decidable_pred M.start
+@[reducible] def step_dec (M : NFA) := Π (S : M.state) (a : M.alphabet), decidable_pred (M.step S a)
 
 instance fin₁ (M : NFA) : fintype M.alphabet := M.alphabet_fintype
 instance fin₂ (M : NFA) : fintype M.state := M.state_fintype
@@ -24,7 +24,7 @@ instance fin₂ (M : NFA) : fintype M.state := M.state_fintype
 def step_set (M : NFA) : set M.state → M.alphabet → set M.state :=
 λ Ss a, Ss >>= λ S, M.step S a
 
-instance step_set_dec (M : NFA) (a : M.alphabet) :
+instance step_set_dec (M : NFA) (a : M.alphabet) [M.step_dec] :
 Π (Ss : set M.state) [decidable_pred Ss], decidable_pred (M.step_set Ss a) :=
 begin
   intro Ss,
@@ -41,39 +41,32 @@ end
 
 def eval (M : NFA) : list M.alphabet → set M.state := list.foldl M.step_set M.start
 
-instance eval_dec (M : NFA) (s : list M.alphabet) : decidable_pred (M.eval s) :=
+instance eval_dec (M : NFA) (s : list M.alphabet) [hdec : M.start_dec] [M.step_dec] : 
+decidable_pred (M.eval s) :=
 begin
   rw eval,
-  have hdec := M.start_dec,
+  tactic.unfreeze_local_instances,
   revert hdec,
+  change Π [hdec : decidable_pred M.start], decidable_pred (list.foldl M.step_set M.start s),
   generalize : M.start = start,
   revert start,
-  induction s with a s ih,
-  { intros _ _, 
-    rw list.foldl,
-    assumption },
-  { intro start, 
-    introI hdec,
-    rw list.foldl,
-    specialize ih (M.step_set start a),
-    exact ih (M.step_set_dec a start) }
+  induction s with a s ih;
+  tauto
 end
 
 def accepts (M : NFA) (s : list M.alphabet) : Prop :=
 ∃ S ∈ M.accept_states, S ∈ M.eval s
 
-def NFA_of_DFA (M : DFA) [decidable_eq M.state] : NFA :=
+def NFA_of_DFA (M : DFA) : NFA :=
 { alphabet := M.alphabet,
   alphabet_fintype := M.alphabet_fintype,
   state := M.state,
   state_fintype := M.state_fintype,
   step := λ S a, {M.step S a},
-  step_dec := by tauto,
   start := {M.start},
-  start_dec := by tauto,
   accept_states := M.accept_states }
 
-lemma NFA_of_DFA_eval_match (M : DFA) [decidable_eq M.state] (s : list M.alphabet) :
+lemma NFA_of_DFA_eval_match (M : DFA) (s : list M.alphabet) :
   {M.eval s} = (NFA_of_DFA M).eval s :=
 begin
   change {list.foldl M.step M.start s} = list.foldl (NFA_of_DFA M).step_set {M.start} s,
@@ -85,13 +78,12 @@ begin
     rw [list.foldl, list.foldl],
     have : (NFA_of_DFA M).step_set {start} a = {M.step start a},
     { rw step_set,
-      simp only [set.bUnion_singleton, set.bind_def],
-      tauto },
+      finish },
     rw this,
     tauto }
 end
 
-lemma NFA_of_DFA_correct (M : DFA) [decidable_eq M.state] (s : list M.alphabet) :
+lemma NFA_of_DFA_correct (M : DFA) (s : list M.alphabet) :
   M.accepts s ↔ (NFA_of_DFA M).accepts s :=
 begin
   rw [accepts, DFA.accepts, ←NFA_of_DFA_eval_match],
